prove Los_modal_thm according to https://www.phil.pku.edu.cn/personal/wangyj/files/Teaching/AML/18Slides/Basic10UP.pdf

FOLModelScript.sml
@@ -4,31 +4,250 @@ open FOLSyntaxTheory;
 
 val _ = new_theory "FOLModel";
 
-(*
 
-val _ = Datatype`
-        folmodel = <| domain : 'a set ;
-	              consts : num -> 'a;
-	              fnsyms : num -> 'a list -> 'a;
-		      predsyms : 'p -> 'a -> bool;
-		      relsyms : 'p -> 'a -> 'a -> bool;
-		      |>`;
+val models2worlds_def = Define`
+  models2worlds MS = \i. (MS i).domain`;
 
-val interpret_def = Define`
-  interpret M σ (fVar n) = σ n /\
-  interpret M σ (fConst n) = M.consts n`;
+val ultraproduct_model_def = Define`
+!U I MS.
+      ultraproduct_model U I MS =
+      <| domain := ultraproduct_model U I (models2worlds MS);
+         consts := \n. 
+	 fnsyms := \x y. ARB;
+	 predsyms := \p 
 
 
-val Models_def = Define`
-  Models M σ (fPrel a t) = M.predsyms a (interpret M σ t) /\
-  Models M σ (fRrel a t1 t2) = M.relsyms a (interpret M σ t1) (interpret M σ t2) /\
-  Models M σ (fDISJ f1 f2) = (Models M σ f1 \/  Models M σ f2) /\
-  Models M σ (fNOT f) = ¬(Models M σ f) /\
-  Models M σ (fEXISTS n f) = (?x. x IN M.domain /\ Models M ((n=+x)σ) f) /\
-  Models M σ (fEQ t1 t2) = (interpret M σ t1 = interpret M σ t2)`;
 
 
-*)
+
+
+
+
+
+
+frame :=
+          <|world := ultraproduct U I (models2worlds MS);
+            rel :=
+              (\fu gu.
+                  ?f g.
+                     f IN fu /\ g IN gu /\
+                     {i | i IN I /\ (MS i).frame.rel (f i) (g i)} IN
+                     U)|>;
+        valt :=
+          (\p fu.
+              ?f.
+                 f IN fu /\ {i | i IN I /\ f i IN (MS i).valt p} IN U)|>
+
+
+
+
+
+val ultrafilter_theorem = store_thm(
+"ultrafilter_theorem",
+``!f w. proper_filter f w ==> ?U. ultrafilter U w /\ f SUBSET U``,
+rpt strip_tac >>
+qabbrev_tac
+  `r = { (s1,s2) | proper_filter s2 w /\ proper_filter s1 w /\ f SUBSET s1 /\ s1 ⊆ s2}` >>
+qabbrev_tac `s = { g | proper_filter g w /\ f ⊆ g }` >>
+`partial_order r s`
+  by (simp[Abbr`r`, Abbr`s`, partial_order_def, reflexive_def, transitive_def,
+           domain_def, range_def] >> rw[] >> simp[]
+      >- (rw[SUBSET_DEF] >> metis_tac[])
+      >- (rw[SUBSET_DEF] >> metis_tac[])
+      >- metis_tac[SUBSET_TRANS]
+      >- (simp[antisym_def] >> rw[] >> fs[] >> metis_tac[SUBSET_ANTISYM])) >>
+`s ≠ ∅` by (simp[EXTENSION, Abbr`s`] >> metis_tac[SUBSET_REFL]) >>
+`∀t. chain t r ==> upper_bounds t r ≠ ∅`
+  by (rw[] >> Cases_on `t = {}`
+        >- (simp[chain_def, upper_bounds_def, Abbr`r`] >> rw[] >>
+            simp[Once EXTENSION] >>
+            qexists_tac `f` >>
+            simp[range_def] >> qexists_tac `f` >> rw[])
+        >- (simp[chain_def, upper_bounds_def, Abbr`r`] >> rw[] >>
+            simp[Once EXTENSION] >>
+            qexists_tac `BIGUNION t` >> rw[]
+          >- (* BIGUNION is in (range of) relation *)
+             (* BIGUNION is proper filter *)
+	     (simp[range_def] >> qexists_tac `f` >> rw[]
+	     (* is proper filter *)
+	    >- (irule UNION_proper_proper
+	      >- (fs[chain_def] >> metis_tac[])
+	      >- (fs[chain_def] >> metis_tac[])
+	      >- metis_tac[proper_filter_def,filter_def]
+	      >- rw[])
+             (* contain f *)
+	    >- (fs[chain_def,Abbr`s`] >> rw[SUBSET_DEF] >>
+	      `?a. a IN t` by metis_tac[MEMBER_NOT_EMPTY] >> qexists_tac `a` >> rw[] >> metis_tac[SUBSET_DEF]))
+             (* indeed upper bound *)
+          >- (`y IN t ==> proper_filter (BIGUNION t) w ∧ proper_filter y w ∧ f ⊆ y ∧ y ⊆ BIGUNION t` suffices_by metis_tac[] >> rw[]
+	    >- (irule UNION_proper_proper >> rw[]
+	        >- (fs[chain_def] >> metis_tac[])
+	        >- (fs[chain_def] >> metis_tac[])
+	        >- metis_tac[proper_filter_def,filter_def])
+	    >- (fs[chain_def] >> metis_tac[])
+	    >- (fs[chain_def] >> metis_tac[])
+	    >- (rw[SUBSET_DEF,BIGUNION] >> metis_tac[])))) >>
+ `?x. x IN maximal_elements s r` by metis_tac[zorns_lemma] >>
+ fs[maximal_elements_def,Abbr`r`,Abbr`s`] >> qexists_tac `x` >> rw[] >>
+ irule maximal_ultrafilter >> rw[] >> SPOSE_NOT_THEN ASSUME_TAC >>
+ `proper_filter S' w` by metis_tac[proper_filter_def] >>
+ `x <> S'` by metis_tac[PSUBSET_DEF] >>
+ `x = S'` by (first_x_assum irule >> fs[] (* 2 *)
+ >> metis_tac[PSUBSET_DEF,SUBSET_TRANS]));
+
+
+val fvars_def = Define`
+  fvars (fRrel a t1 t2) = tvars t1 ∪ tvars t2 /\
+  fvars (fPrel a t) = tvars t /\
+  fvars (fDISJ ff1 ff2) = (fvars ff1) ∪ (fvars ff2) /\
+  fvars (fNOT ff) = fvars ff /\
+  fvars (fEXISTS n ff) = n INSERT (fvars ff) /\
+  fvars (fEQ t1 t2) = tvars t1 ∪ tvars t2`;
+
+val qfree_def = Define`
+    (qfree (fRrel a t1 t2) = T) /\
+    (qfree (fPrel a t) = T) /\
+    (qfree (fDISJ ff1 ff2) = (qfree ff1 /\ qfree ff2)) /\
+    (qfree (fNOT ff) = qfree ff) /\
+    (qfree (fEXISTS n ff) = F) /\
+    (qfree (fEQ t1 t2) = T)`;
+
+
+val psatisfiable_def = Define`
+  psatisfiable ss (μ:'a itself) (ν:'b itself) = ?M:('a,'b,unit)folmodel σ. (!f. f IN ss ==> fsatis M σ f)`;
+
+val finsat_def = Define`
+  finsat ss (μ:'a itself) (ν:'b itself) = (!s0. s0 ⊆ ss /\ FINITE s0 ==> psatisfiable s0 μ ν)`;
+
+
+val FINITE_chain_SUBSET_lemma = store_thm(
+  "FINITE_chain_SUBSET_lemma",
+  ``(!A B. A IN U /\ B IN U ==> A ⊆ B \/ B ⊆ A) ==> 
+
+val UNION_finsat_finsat = store_thm(
+  "UNION_finsat_finsat",
+  ``!U. (!A. A IN U ==> finsat A μ ν) /\ (!A B. A IN U /\ B IN U ==> A ⊆ B \/ B ⊆ A) ==> finsat (BIGUNION U) μ ν``,
+  rw[finsat_def,psatisfiable_def,BIGUNION] >>
+  `!f. f IN s0 ==> ?s. s IN U /\ f IN s` by (rw[] >> fs[SUBSET_DEF]) >>
+  qabbrev_tac `ss = {u | ?f. f IN s0 /\ u = CHOICE {u0 | u0 IN U /\ f IN u0}}` >>
+  Cases_on `s0 = {}` >> rw[] >> 
+  `(BIGUNION ss) IN U`
+      by (rw[Abbr`ss`] >>
+         `!s0. FINITE s0 ==>
+         s0 SUBSET {x | ?s. s IN U /\ x IN s} /\ (!f. f IN s0 ==> ?s. s IN U /\ f IN s) /\ s0 <> {} ==>
+	 BIGUNION {u | ?f. f IN s0 /\ u = CHOICE {u0 | u0 IN U /\ f IN u0}} IN U` suffices_by metis_tac[] >>
+         Induct_on `FINITE` >> rw[] >> Cases_on `s0' = {}` >> rw[] (* 2 *)
+ >- (`{u0 | u0 IN U /\ e IN u0} <> {}`
+      by (`?u. u IN {u0 | u0 IN U /\ e IN u0}` suffices_by metis_tac[MEMBER_NOT_EMPTY] >>
+         qexists_tac `s` >> fs[]) >>
+    `(CHOICE {u0 | u0 IN U /\ e IN u0}) IN {u0 | u0 IN U /\ e IN u0}` by metis_tac[CHOICE_DEF] >> fs[])
+ >- (`(!f. f IN s0' ==> ?s. s IN U /\ f IN s)` by metis_tac[] >>
+    `BIGUNION {u | ?f. f IN s0' /\ u = CHOICE {u0 | u0 IN U /\ f IN u0}} IN U` by metis_tac[] >>
+    `BIGUNION {u | ?f. (f = e \/ f IN s0') /\ u = CHOICE {u0 | u0 IN U /\ f IN u0}} =
+    (CHOICE {u0 | u0 IN U /\ e IN u0}) ∪
+    (BIGUNION {u | ?f. f IN s0' /\ u = CHOICE {u0 | u0 IN U /\ f IN u0}})`
+      by (rw[EXTENSION,EQ_IMP_THM,BIGUNION,PULL_EXISTS] >> metis_tac[]) >>
+    `(CHOICE {u0 | u0 IN U /\ e IN u0}) IN U`
+      by (`{u0 | u0 IN U /\ e IN u0} <> {}`
+            by (`?u. u IN {u0 | u0 IN U /\ e IN u0}` suffices_by metis_tac[MEMBER_NOT_EMPTY] >>
+	       qexists_tac `s` >> fs[]) >>
+    `(CHOICE {u0 | u0 IN U /\ e IN u0}) IN {u0 | u0 IN U /\ e IN u0}` by metis_tac[CHOICE_DEF] >> fs[]) >>
+    Cases_on `CHOICE {u0 | u0 IN U /\ e IN u0} ⊆
+             BIGUNION {u | ?f. f IN s0' /\ u = CHOICE {u0 | u0 IN U /\ f IN u0}}`
+    >- (`CHOICE {u0 | u0 IN U /\ e IN u0} UNION
+       BIGUNION
+         {u | ?f. f IN s0' /\ u = CHOICE {u0 | u0 IN U /\ f IN u0}} =
+       BIGUNION
+         {u | ?f. f IN s0' /\ u = CHOICE {u0 | u0 IN U /\ f IN u0}}` by metis_tac[SUBSET_UNION_ABSORPTION] >>
+       metis_tac[])
+    >- (`BIGUNION {u | ?f. f IN s0' /\ u = CHOICE {u0 | u0 IN U /\ f IN u0}} ⊆ CHOICE {u0 | u0 IN U /\ e IN u0}`
+       by metis_tac[] >>
+       `CHOICE {u0 | u0 IN U /\ e IN u0} UNION
+       BIGUNION
+         {u | ?f. f IN s0' /\ u = CHOICE {u0 | u0 IN U /\ f IN u0}} = CHOICE {u0 | u0 IN U /\ e IN u0}`
+         by metis_tac[SUBSET_UNION_ABSORPTION,UNION_COMM] >> metis_tac[]))) >>
+  `s0 ⊆ (BIGUNION ss)`
+    by (rw[BIGUNION,SUBSET_DEF,Abbr`ss`,PULL_EXISTS] >> qexists_tac `x` >> rw[] >>
+       `{u0 | u0 IN U /\ x IN u0} <> {}`
+         by (`x IN {x | ?s. s IN U /\ x IN s}` by metis_tac[SUBSET_DEF] >>
+	    fs[] >> `?t. t IN {u0 | u0 IN U /\ x IN u0}` suffices_by metis_tac[MEMBER_NOT_EMPTY] >>
+	    qexists_tac `s` >> fs[]) >>
+       `(CHOICE {u0 | u0 IN U /\ x IN u0}) IN {u0 | u0 IN U /\ x IN u0}` by metis_tac[CHOICE_DEF] >>
+       fs[]) >>
+  metis_tac[]);
+  
+
+
+val finsat_extension_lemma = store_thm(
+  "finsat_extension_lemma",
+  ``finsat A μ ν ==> ?B. A ⊆ B /\ finsat B μ ν /\
+                     (!C. B ⊆ C /\ finsat C μ ν ==> C = B)``,
+  rw[] >>
+  qabbrev_tac
+  `r = { (s1,s2) | finsat s1 μ ν /\ finsat s2 μ ν /\ A ⊆ s1 /\ s1 ⊆ s2}` >>
+  qabbrev_tac `s = { g | finsat g μ ν /\ A ⊆ g }` >>
+  `partial_order r s`
+  by (simp[Abbr`r`, Abbr`s`, partial_order_def, reflexive_def, transitive_def,
+           domain_def, range_def] >> rw[] >> simp[]
+      >- (rw[SUBSET_DEF] >> metis_tac[])
+      >- (rw[SUBSET_DEF] >> metis_tac[])
+      >- metis_tac[SUBSET_TRANS]
+      >- (simp[antisym_def] >> rw[] >> fs[] >> metis_tac[SUBSET_ANTISYM])) >>
+  `s ≠ ∅` by (simp[EXTENSION, Abbr`s`] >> metis_tac[SUBSET_REFL]) >>
+  `∀t. chain t r ==> upper_bounds t r ≠ ∅`
+    by (rw[] >> Cases_on `t = {}`
+        >- (simp[chain_def, upper_bounds_def, Abbr`r`] >> rw[] >>
+            simp[Once EXTENSION] >>
+            qexists_tac `A` >>
+            simp[range_def] >> qexists_tac `A` >> rw[])
+        >- (simp[chain_def, upper_bounds_def, Abbr`r`] >> rw[] >>
+            simp[Once EXTENSION] >>
+            qexists_tac `BIGUNION t` >> rw[]
+          >- (* BIGUNION is in (range of) relation *)
+             (* BIGUNION is proper filter *)
+	     (simp[range_def] >> qexists_tac `A` >> rw[]
+	     (* is proper filter *)
+	    >- (irule UNION_proper_proper
+	      >- (fs[chain_def] >> metis_tac[])
+	      >- (fs[chain_def] >> metis_tac[])
+	      >- metis_tac[proper_filter_def,filter_def]
+	      >- rw[])
+             (* contain f *)
+	    >- (fs[chain_def,Abbr`s`] >> rw[SUBSET_DEF] >>
+	      `?a. a IN t` by metis_tac[MEMBER_NOT_EMPTY] >> qexists_tac `a` >> rw[] >>
+	      `A ⊆ a` suffices_by metis_tac[SUBSET_DEF] >>
+	      `a IN t /\ a IN t` suffices_by metis_tac[] last_x_assum imp_res_tac
+	      first_x_assum irule
+	      `(finsat a μ ν /\ finsat a μ ν /\ A SUBSET a /\ a SUBSET a) \/
+	      (finsat a μ ν /\ finsat a μ ν /\ A SUBSET a /\ a SUBSET a)` by metis_tac[]))
+             (* indeed upper bound *)
+          >- (`y IN t ==> proper_filter (BIGUNION t) w ∧ proper_filter y w ∧ f ⊆ y ∧ y ⊆ BIGUNION t` suffices_by metis_tac[] >> rw[]
+	    >- (irule UNION_proper_proper >> rw[]
+	        >- (fs[chain_def] >> metis_tac[])
+	        >- (fs[chain_def] >> metis_tac[])
+	        >- metis_tac[proper_filter_def,filter_def])
+	    >- (fs[chain_def] >> metis_tac[])
+	    >- (fs[chain_def] >> metis_tac[])
+	    >- (rw[SUBSET_DEF,BIGUNION] >> metis_tac[])))) >>
+  
+
+
+
+
+
+
+
+
+val thm_A_19 = store_thm(
+  "thm_A_19",
+  ``!ff. fsatis <=> fsati
+
+
+
+
+
+
+
 
 val _ = export_theory();
 
