chap2_7Script.sml
@@ -1,0 +1,77 @@
+open HolKernel Parse boolLib bossLib;
+open chap1Theory;
+open pred_setTheory;
+open relationTheory;
+open arithmeticTheory;
+open set_relationTheory;
+
+open chap2_1Theory;
+open chap2_2Theory;
+open chap2_4revisedTheory;
+open chap2_5Theory
+open equiv_on_partitionTheory;
+open IBCDNFrevisedTheory;
+open prim_recTheory;
+open listTheory;
+open finite_mapTheory;
+open combinTheory;
+
+val _ = ParseExtras.tight_equality()
+
+val _ = new_theory "chap2_7";
+
+
+val sim_def = Define`
+  sim Z M M' <=>
+  !w w'. w IN M.frame.world /\ w' IN M'.frame.world /\ Z w w' ==>
+  (!p. w IN M.valt p ==> w' IN M'.valt p) /\
+  (!v. v IN M.frame.world /\ M.frame.rel w v ==> ?v'. v' IN M'.frame.world /\ Z v v' /\ M'.frame.rel w' v')`;
+
+val preserved_under_sim_def = Define`
+  preserved_under_sim (μ:'a itself) (ν:'b itself) phi <=> 
+  (!M M' Z w w'. w:'a IN M.frame.world /\ w':'b IN M'.frame.world /\ sim Z M M' /\ Z w w' ==> (satis M w phi ==> satis M' w' phi))`;
+
+
+
+val (PE_rules, PE_ind, PE_cases) = Hol_reln`
+  (!p. PE (VAR p)) /\ 
+  (!f1 f2. (PE f1 /\ PE f2) ==> PE (AND f1 f2)) /\ 
+  (!f1 f2. (PE f1 /\ PE f2) ==> PE (DISJ f1 f2)) /\
+  (!f. PE f ==> PE (DIAM f))`;    
+
+
+val thm_2_78_half1_lemma = store_thm(
+  "thm_2_78_half1_lemma",
+  ``!phi. PE phi ==> (!μ ν. preserved_under_sim μ ν phi)``,
+   Induct_on `PE phi` >> rw[preserved_under_sim_def] (* 4 *)
+   >- (fs[satis_def] >> metis_tac[sim_def])
+   >- (fs[satis_AND] >> metis_tac[])
+   >- (fs[satis_def] >> metis_tac[])
+   >- (fs[satis_def] >> imp_res_tac sim_def >> metis_tac[]));
+
+val thm_2_78_half1 = store_thm(
+  "thm_2_78_half1",
+  ``!phi phi0 μ ν. (PE phi0 /\ equiv0 μ phi phi0 /\ equiv0 ν phi phi0) ==> preserved_under_sim μ ν phi``,
+  rw[] >> `preserved_under_sim μ ν phi0` by metis_tac[thm_2_78_half1_lemma] >>
+  fs[preserved_under_sim_def] >> rw[] >> fs[equiv0_def] >> `satis M w phi0` by metis_tac[] >> metis_tac[]);
+
+
+ Let  be a set of ﬁrst-order formulas. If each ﬁnite subset of  has a model, then  itself has a model.
+
+
+val compactness_theorem = store_thm(
+  "compactness_theorem",
+  ``!Σ. (!Σ0. FINITE Σ0 /\ Σ0 ⊆ Σ ==> (?M σ. !f. f IN Σ0 ==> fsatis M σ f)) ==>
+         ?M σ. (!f. f IN Σ ==> fsatis M σ f)``,
+  
+
+  
+  
+
+val thm_2_78_half2 = store_thm(
+  "thm_2_78_half2",
+  ``!phi μ ν. preserved_under_sim μ ν phi ==> (?phi0. equiv0 μ phi phi0 /\ equiv0 ν phi phi0 /\ PE phi0)``,
+  rw[] >>
+
+
+  
