ultraproductScript.sml
@@ -32,8 +32,14 @@ val prop_A_16 = store_thm(
      `{i | i ∈ I' ∧ x i = z i} ⊆ I'` by rw[SUBSET_DEF] >>
      metis_tac[ultrafilter_def,proper_filter_def,filter_def]));
 
+
+
+
 val ultraproduct_def = Define`
   ultraproduct U I A = partition (Uequiv U I A) (Cart_prod I A)`;
+
+
+(*
 
 val models2worlds_def = Define`
   models2worlds MS = \i. (MS i).frame.world`;
@@ -44,87 +50,434 @@ val ultraproduct_model_def = Define`
 					                      {i | i IN I /\ (MS i).frame.rel (f i) (g i)} IN U) |>;
 			          valt := \p fu. (?f. f IN fu /\ {i | i IN I /\ (f i) IN (MS i).valt p} IN U) |>`;
 
+
+val ultrapower_valt_well_defined = store_thm(
+  "ultrapower_valt_well_defined",
+  ``!U J Ms. ultrafilter U J ==> !f g. Uequiv U J (models2worlds Ms) f g ==>
+             ({i | i IN J /\ (f i) IN (Ms i).valt p} IN U <=>
+	     {i | i IN J /\ (g i) IN (Ms i).valt p} IN U)``,
+  rw[Uequiv_def,models2worlds_def,Cart_prod_def] >> eq_tac >> rw[]
+  >- (`{i | i IN J /\ f i = g i} ∩ {i | i IN J /\ f i IN (Ms i).valt p} IN U`
+       by metis_tac[ultrafilter_def,proper_filter_def,filter_def] >>
+     `{i | i IN J /\ g i IN (Ms i).valt p} ⊆ J` by fs[SUBSET_DEF] >>
+     `({i | i IN J /\ f i = g i} ∩ {i | i IN J /\ f i IN (Ms i).valt p}) ⊆
+     {i | i IN J /\ g i IN (Ms i).valt p}` suffices_by metis_tac[ultrafilter_def,proper_filter_def,filter_def] >>
+     rw[INTER_DEF,SUBSET_DEF] >> metis_tac[])
+  >- (`{i | i IN J /\ f i = g i} ∩ {i | i IN J /\ g i IN (Ms i).valt p} IN U`
+       by metis_tac[ultrafilter_def,proper_filter_def,filter_def] >>
+     `{i | i IN J /\ f i IN (Ms i).valt p} ⊆ J` by fs[SUBSET_DEF] >>
+     `({i | i IN J /\ f i = g i} ∩ {i | i IN J /\ g i IN (Ms i).valt p}) ⊆
+     {i | i IN J /\ f i IN (Ms i).valt p}` suffices_by metis_tac[ultrafilter_def,proper_filter_def,filter_def] >>
+     rw[INTER_DEF,SUBSET_DEF] >> metis_tac[]));
+
+val Los_modal_thm = store_thm(
+  "Los_modal_thm",
+  ``!U J Ms. ultrafilter U J ==>
+             !phi fc. (satis (ultraproduct_model U J Ms) fc phi <=>
+	              (fc IN (ultraproduct_model U J Ms).frame.world /\
+	              ?f. f IN fc /\ {i | i IN J /\ satis (Ms i) (f i) phi} IN U))``,
+  strip_tac >> strip_tac >> strip_tac  >> strip_tac >> Induct_on `phi` >> rw[]
+  >- (rw[satis_def,ultraproduct_world,ultraproduct_valt] >> eq_tac >> rw[]
+     >> qexists_tac `f` >> rw[] >> fs[] >>
+        `{i | i IN J /\ f i IN (Ms i).frame.world /\ f i IN (Ms i).valt a} =
+	{i | i IN J /\ f i IN (Ms i).valt a}` suffices_by metis_tac[] >>
+	simp[EXTENSION] >> rw[] >> eq_tac >> rw[])
+  >- (rw[satis_def,EQ_IMP_THM,ultraproduct_world] (* 7 *)
+     >- metis_tac[]
+     >- (qexists_tac `x` >> rw[])
+     >- (qexists_tac `f` >> rw[] >> 
+        `{i | i IN J /\ (satis (Ms i) (f i) phi \/ satis (Ms i) (f i) phi')} ⊆ J` by fs[SUBSET_DEF] >>
+	`{i | i IN J /\ satis (Ms i) (f i) phi} ⊆ {i | i IN J /\ (satis (Ms i) (f i) phi \/ satis (Ms i) (f i) phi')}` suffices_by metis_tac[ultrafilter_def,proper_filter_def,filter_def] >> fs[SUBSET_DEF])
+     >- metis_tac[]
+     >- (qexists_tac `x` >> rw[])
+     >- (qexists_tac `f` >> rw[] >> 
+        `{i | i IN J /\ (satis (Ms i) (f i) phi \/ satis (Ms i) (f i) phi')} ⊆ J` by fs[SUBSET_DEF] >>
+	`{i | i IN J /\ satis (Ms i) (f i) phi'} ⊆ {i | i IN J /\ (satis (Ms i) (f i) phi \/ satis (Ms i) (f i) phi')}` suffices_by metis_tac[ultrafilter_def,proper_filter_def,filter_def] >> fs[SUBSET_DEF])
+     >- (`{i | i IN J /\ (satis (Ms i) (f i) phi \/ satis (Ms i) (f i) phi')} =
+        {i | i IN J /\ satis (Ms i) (f i) phi} ∪ {i | i IN J /\ satis (Ms i) (f i) phi'}`
+	  by (rw[EXTENSION,EQ_IMP_THM] >> metis_tac[]) >>
+	`{i | i IN J /\ satis (Ms i) (f i) phi} ⊆ J /\
+	 {i | i IN J /\ satis (Ms i) (f i) phi'} ⊆ J` by fs[SUBSET_DEF] >>
+	`{i | i IN J /\ satis (Ms i) (f i) phi} IN U \/
+	{i | i IN J /\ satis (Ms i) (f i) phi'} IN U` by metis_tac[ultrafilter_UNION]
+	>> metis_tac[]))
+  >- (rw[satis_def] >> metis_tac[EMPTY_NOTIN_ultrafilter])
+  >- rw[satis_def,EQ_IMP_THM,ultraproduct_world]
+     >- metis_tac[]
+     >- metis_tac[]
+     >- qexists_tac `f` >> rw[] >>
+        `f NOTIN
+         {y |
+          (!i. i IN J ==> y i IN (Ms i).frame.world) /\
+          {i | i IN J /\ x i = y i} IN U} \/
+         {i | i IN J /\ satis (Ms i) (f i) phi} NOTIN U` by metis_tac[]
+
+
+fs[ultraproduct_world]
+
+
+val Los_modal_thm = store_thm(
+  "Los_modal_thm",
+  ``!U J Ms. ultrafilter U J ==>
+             !phi fc. fc IN (ultraproduct_model U J Ms).frame.world ==>
+	              (satis (ultraproduct_model U J Ms) fc phi <=>
+	              ?f. f IN fc /\ {i | i IN J /\ satis (Ms i) (f i) phi} IN U)``,
+  strip_tac >> strip_tac >> strip_tac  >> strip_tac >> Induct_on `phi` >> rw[] (* 5 *)
+
+
+(*-----------------------------block 1 `` ¬ case``------------------------------------- *)
+rw[satis_def,EQ_IMP_THM,ultraproduct_world] (* 2 *)
+>- (`(!i. i IN J ==> (Ms i).frame.world <> {}) /\
+    ?x. (!i. i IN J ==> x i IN (Ms i).frame.world) /\
+        fc = {y |
+             (!i. i IN J ==> y i IN (Ms i).frame.world) /\
+             {i | i IN J /\ x i = y i} IN U}` by metis_tac[ultraproduct_world] >>
+   qexists_tac `x` >> rw[] (* 2 *)
+   >- metis_tac[ultrafilter_def,proper_filter_def,filter_def]
+   >- (`x IN {y | (!i. i IN J ==> y i IN (Ms i).frame.world) /\ {i | i IN J /\ x i = y i} IN U}`
+        by (rw[] >> metis_tac[ultrafilter_def,proper_filter_def,filter_def]) >>
+      `{i | i IN J /\ satis (Ms i) (x i) phi} NOTIN U` by metis_tac[] >>
+      `{i | i IN J /\ satis (Ms i) (x i) phi} IN (POW J)` by fs[SUBSET_DEF,POW_DEF] >>
+      `J DIFF {i | i IN J /\ satis (Ms i) (x i) phi} IN U` by metis_tac[ultrafilter_def] >>
+      fs[DIFF_DEF] >>
+      `{i | i IN J /\ x i IN (Ms i).frame.world /\ ~satis (Ms i) (x i) phi} =
+      {x' | x' IN J /\ (x' NOTIN J \/ ~satis (Ms x') (x x') phi)}`
+        by rw[EXTENSION,EQ_IMP_THM] >>
+      metis_tac[]))
+>- (`!f'. f' IN fc ==> {i | i IN J /\ satis (Ms i) (f' i) phi} NOTIN U` suffices_by metis_tac[] >> rw[] >>
+   `(!i. i IN J ==> (Ms i).frame.world <> {}) /\
+    ?x. (!i. i IN J ==> x i IN (Ms i).frame.world) /\
+        fc = {y |
+             (!i. i IN J ==> y i IN (Ms i).frame.world) /\
+             {i | i IN J /\ x i = y i} IN U}` by metis_tac[ultraproduct_world] >>
+   fs[] >>
+   `{i | i IN J /\ satis (Ms i) (f' i) phi} IN (POW J)` by fs[SUBSET_DEF,POW_DEF] >>
+   `J DIFF {i | i IN J /\ satis (Ms i) (f' i) phi} IN U` suffices_by metis_tac[ultrafilter_def] >>
+   rw[DIFF_DEF] >>
+   `{x | x IN J /\ (x NOTIN J \/ ~satis (Ms x) (f' x) phi)} =
+   {x | x IN J /\ ~satis (Ms x) (f' x) phi}` by rw[EXTENSION,EQ_IMP_THM] >> fs[] >>
+   `{i | i IN J /\ f i IN (Ms i).frame.world /\ ~satis (Ms i) (f i) phi} ∩
+   {i | i IN J /\ x i = f i} IN U` by metis_tac[ultrafilter_def,proper_filter_def,filter_def] >>
+   `({i | i IN J /\ f i IN (Ms i).frame.world /\ ~satis (Ms i) (f i) phi} ∩
+   {i | i IN J /\ x i = f i}) ∩  {i | i IN J /\ x i = f' i} IN U` by metis_tac[ultrafilter_def,proper_filter_def,filter_def] >>
+   `({i | i IN J /\ f i IN (Ms i).frame.world /\ ~satis (Ms i) (f i) phi} ∩
+   {i | i IN J /\ x i = f i}) ∩  {i | i IN J /\ x i = f' i} ⊆
+   {x | x IN J /\ ~satis (Ms x) (f' x) phi}` by (rw[SUBSET_DEF] >> metis_tac[]) >>
+   `{x | x IN J /\ ~satis (Ms x) (f' x) phi} ⊆ J` by rw[SUBSET_DEF] >>
+   metis_tac[ultrafilter_def,proper_filter_def,filter_def])
+ 
+
+
+(*-----------------------------block 2 `` \/ case``------------------------------------- *)
+rw[satis_def,EQ_IMP_THM,ultraproduct_world] (* 3 *)
+>- (qexists_tac `f` >> rw[] >> 
+        `{i | i IN J /\ (satis (Ms i) (f i) phi \/ satis (Ms i) (f i) phi')} ⊆ J` by fs[SUBSET_DEF] >>
+	`{i | i IN J /\ satis (Ms i) (f i) phi} ⊆ {i | i IN J /\ (satis (Ms i) (f i) phi \/ satis (Ms i) (f i) phi')}` suffices_by metis_tac[ultrafilter_def,proper_filter_def,filter_def] >> fs[SUBSET_DEF])
+>- (qexists_tac `f` >> rw[] >> 
+        `{i | i IN J /\ (satis (Ms i) (f i) phi \/ satis (Ms i) (f i) phi')} ⊆ J` by fs[SUBSET_DEF] >>
+	`{i | i IN J /\ satis (Ms i) (f i) phi'} ⊆ {i | i IN J /\ (satis (Ms i) (f i) phi \/ satis (Ms i) (f i) phi')}` suffices_by metis_tac[ultrafilter_def,proper_filter_def,filter_def] >> fs[SUBSET_DEF])
+>- (`{i | i IN J /\ (satis (Ms i) (f i) phi \/ satis (Ms i) (f i) phi')} =
+        {i | i IN J /\ satis (Ms i) (f i) phi} ∪ {i | i IN J /\ satis (Ms i) (f i) phi'}`
+	  by (rw[EXTENSION,EQ_IMP_THM] >> metis_tac[]) >>
+	`{i | i IN J /\ satis (Ms i) (f i) phi} ⊆ J /\
+	 {i | i IN J /\ satis (Ms i) (f i) phi'} ⊆ J` by fs[SUBSET_DEF] >>
+	`{i | i IN J /\ satis (Ms i) (f i) phi} IN U \/
+	{i | i IN J /\ satis (Ms i) (f i) phi'} IN U` by metis_tac[ultrafilter_UNION]
+	>> metis_tac[])
+
+
+(*-----------------------------block 3 `` VAR case``------------------------------------- *)
+fs[satis_def,ultraproduct_world,ultraproduct_valt] >> eq_tac >> rw[] (* 2 *)
+>- (qexists_tac `f` >> rw[] >> fs[] >>
+        `{i | i IN J /\ f i IN (Ms i).frame.world /\ f i IN (Ms i).valt a} =
+	{i | i IN J /\ f i IN (Ms i).valt a}` suffices_by metis_tac[] >>
+	simp[EXTENSION] >> rw[] >> eq_tac >> rw[] >>
+	`(!i. i IN J ==> (Ms i).frame.world <> {}) /\
+         ?x.
+            (!i. i IN J ==> x i IN (Ms i).frame.world) /\
+            fc =
+            {y |
+             (!i. i IN J ==> y i IN (Ms i).frame.world) /\
+             {i | i IN J /\ x i = y i} IN U}` by metis_tac[ultraproduct_world] >>
+	`f IN {y | (!i. i IN J ==> y i IN (Ms i).frame.world) /\ {i | i IN J /\ x' i = y i} IN U}`
+	  by metis_tac[] >> fs[])
+>- (`(!i. i IN J ==> (Ms i).frame.world <> {}) /\
+   ?x. (!i. i IN J ==> x i IN (Ms i).frame.world) /\
+       fc = {y | (!i. i IN J ==> y i IN (Ms i).frame.world) /\ {i | i IN J /\ x i = y i} IN U}`
+     by metis_tac[ultraproduct_world] >>
+   fs[] >> qexists_tac `f` >> rw[] >>
+   `{i | i IN J /\ f i IN (Ms i).frame.world /\ f i IN (Ms i).valt a} = {i | i IN J /\ f i IN (Ms i).valt a}`
+     by rw[EXTENSION,EQ_IMP_THM] >>
+   metis_tac[])
+
+
+
+
+(*-----------------------------block 4 `` FALSE case``------------------------------------- *)
+`((satis (ultraproduct_model U J Ms) fc FALSE) = F) /\
+((?f. f IN fc /\ {i | i IN J /\ satis (Ms i) (f i) FALSE} IN U) = F)` suffices_by metis_tac[] >> rw[] (* 2 *)
+>- rw[satis_def]
+>- (`{i | i IN J /\ satis (Ms i) (f i) FALSE} NOTIN U` suffices_by metis_tac[] >>
+   `{i | i IN J /\ satis (Ms i) (f i) FALSE} = {}`
+     by rw[EXTENSION,EQ_IMP_THM,satis_def] >>
+   metis_tac[EMPTY_NOTIN_ultrafilter])
+
+
+
+
+
+
+
+
+(*-----------------------------block 4 ``DIAM case``------------------------------------- *)
+rw[satis_def,EQ_IMP_THM,ultraproduct_world] (* 2 *)
+
+
+(*-------------------------------half 1---------------------------------------------------*)
+>- `(!i. i IN J ==> (Ms i).frame.world <> {}) /\
+   ?x. (!i. i IN J ==> x i IN (Ms i).frame.world) /\
+   fc = {y | (!i. i IN J ==> y i IN (Ms i).frame.world) /\ {i | i IN J /\ x i = y i} IN U}` by metis_tac[ultraproduct_world] >> qexists_tac `x'` >> rw[] >> fs[] (* 2 *)
+  >- metis_tac[ultrafilter_def,proper_filter_def,filter_def]
+  >- (`?f g.
+      f IN {y |
+         (!i. i IN J ==> y i IN (Ms i).frame.world) /\
+         {i | i IN J /\ x' i = y i} IN U} /\ g IN {y |
+         (!i. i IN J ==> y i IN (Ms i).frame.world) /\
+         {i | i IN J /\ x i = y i} IN U} /\
+      {i | i IN J /\ (Ms i).frame.rel (f i) (g i)} IN U` by metis_tac[ultraproduct_rel] >> fs[] >>
+     `{i | i IN J /\ x' i = f i} ∩ {i | i IN J /\ (Ms i).frame.rel (f i) (g i)} IN U`
+       by metis_tac[ultrafilter_def,proper_filter_def,filter_def] >>
+     `{i | i IN J /\ x' i = f i} INTER {i | i IN J /\ (Ms i).frame.rel (f i) (g i)} ⊆ {i | i IN J /\ (Ms i).frame.rel (x' i) (g i)} `
+       by rw[SUBSET_DEF] >>
+     `{i | i IN J /\ (Ms i).frame.rel (x' i) (g i)} ⊆ J` by fs[SUBSET_DEF] >>
+     `{i | i IN J /\ (Ms i).frame.rel (x' i) (g i)} IN U` by metis_tac[ultrafilter_def,proper_filter_def,filter_def] >>
+     `{i | i IN J /\ satis (Ms i) (g i) phi} IN U`
+       by (`?r. r IN {y |
+          (!i. i IN J ==> y i IN (Ms i).frame.world) /\
+          {i | i IN J /\ x i = y i} IN U} /\ {i | i IN J /\ satis (Ms i) (r i) phi} IN U` by metis_tac[satis_in_world] >> fs[] >> `{i | i IN J /\ satis (Ms i) (r i) phi} ∩ {i | i IN J /\ x i = r i} IN U` by metis_tac[ultrafilter_def,proper_filter_def,filter_def] >>
+	  `{i | i IN J /\ satis (Ms i) (r i) phi} INTER {i | i IN J /\ x i = r i} ⊆ {i | i IN J /\ satis (Ms i) (x i) phi}` by fs[SUBSET_DEF] >>
+	  `{i | i IN J /\ satis (Ms i) (x i) phi} ⊆ J` by fs[SUBSET_DEF] >>
+	  `{i | i IN J /\ satis (Ms i) (x i) phi} IN U` by metis_tac[ultrafilter_def,proper_filter_def,filter_def] >>
+	  `{i | i IN J /\ g i = x i} = {i | i IN J /\ x i = g i}` by rw[EXTENSION,EQ_IMP_THM] >>
+	  `{i | i IN J /\ satis (Ms i) (x i) phi} INTER {i | i IN J /\ g i = x i} IN U` by metis_tac[ultrafilter_def,proper_filter_def,filter_def] >>
+	  `{i | i IN J /\ satis (Ms i) (x i) phi} INTER {i | i IN J /\ g i = x i} ⊆ {i | i IN J /\ satis (Ms i) (g i) phi}` by fs[SUBSET_DEF] >>
+	  `{i | i IN J /\ satis (Ms i) (g i) phi} ⊆ J` by fs[SUBSET_DEF] >>
+	  metis_tac[ultrafilter_def,proper_filter_def,filter_def]) >>
+     `{i | i IN J /\ (Ms i).frame.rel (x' i) (g i)} ∩ {i | i IN J /\ satis (Ms i) (g i) phi} IN U`
+       by metis_tac[ultrafilter_def,proper_filter_def,filter_def] >>
+     `{i | i IN J /\ (Ms i).frame.rel (x' i) (g i) /\ satis (Ms i) (g i) phi} =
+     {i | i IN J /\ (Ms i).frame.rel (x' i) (g i)} ∩ {i | i IN J /\ satis (Ms i) (g i) phi}`
+       by rw[EXTENSION,EQ_IMP_THM] >>
+     `{i | i IN J /\ (Ms i).frame.rel (x' i) (g i) /\ satis (Ms i) (g i) phi} ⊆
+     {i | i IN J /\ x' i IN (Ms i).frame.world /\
+     ?v. (Ms i).frame.rel (x' i) v /\ v IN (Ms i).frame.world /\ satis (Ms i) v phi}`
+       by (rw[SUBSET_DEF] >> qexists_tac `g x''` >> rw[]) >>
+     `{i | i IN J /\ x' i IN (Ms i).frame.world /\
+      ?v. (Ms i).frame.rel (x' i) v /\ v IN (Ms i).frame.world /\ satis (Ms i) v phi} ⊆ J` by fs[SUBSET_DEF] >>
+      metis_tac[ultrafilter_def,proper_filter_def,filter_def])
+
+
+
+
+
+(*-------------------------------half 2---------------------------------------------------*)
+
+  >- `{i | i IN J /\ f i IN (Ms i).frame.world /\
+      ?v. (Ms i).frame.rel (f i) v /\ v IN (Ms i).frame.world /\ satis (Ms i) v phi} <> {}`
+        by metis_tac[EMPTY_NOTIN_ultrafilter] >> fs[GSYM MEMBER_NOT_EMPTY] >>
+     simp[PULL_EXISTS] >> rw[ultraproduct_rel] >>
+     `?x g. (f IN fc /\
+     ((!i. i IN J ==> g i IN (Ms i).frame.world) /\
+     {i | i IN J /\ x i = g i} IN U) /\
+     {i | i IN J /\ (Ms i).frame.rel (f i) (g i)} IN U) /\
+     (!i. i IN J ==> (Ms i).frame.world <> {}) /\
+     (!i. i IN J ==> x i IN (Ms i).frame.world) /\
+     satis (ultraproduct_model U J Ms)
+     {y | (!i. i IN J ==> y i IN (Ms i).frame.world) /\ {i | i IN J /\ x i = y i} IN U} phi`
+     suffices_by (rw[] >> qexists_tac `x'` >> rw[] (* 2 *)
+                 >- (map_every qexists_tac [`f`,`g`] >> rw[])
+		 >- metis_tac[MEMBER_NOT_EMPTY]) >>
+
+     
+
+
+     map_every qexists_tac
+     [`\i. if (?v.
+          (Ms i).frame.rel (f i) v /\ v IN (Ms i).frame.world /\
+          satis (Ms i) v phi) then CHOICE {v | (Ms i).frame.rel (f i) v /\ v IN (Ms i).frame.world /\ satis (Ms i) v phi}
+	  else CHOICE (Ms i).frame.world`,
+     `\i. if (?v.
+          (Ms i).frame.rel (f i) v /\ v IN (Ms i).frame.world /\
+          satis (Ms i) v phi) then CHOICE {v | (Ms i).frame.rel (f i) v /\ v IN (Ms i).frame.world /\ satis (Ms i) v phi}
+	  else CHOICE (Ms i).frame.world`]>> rw[] (* 8 *)
+     >- (`{v | (Ms i).frame.rel (f i) v /\ v IN (Ms i).frame.world /\ satis (Ms i) v phi} <> {}`
+          by (`v' IN {v | (Ms i).frame.rel (f i) v /\ v IN (Ms i).frame.world /\ satis (Ms i) v phi}` by fs[] >>
+	     metis_tac[MEMBER_NOT_EMPTY]) >>
+	`CHOICE {v | (Ms i).frame.rel (f i) v /\ v IN (Ms i).frame.world /\ satis (Ms i) v phi} IN
+	{v | (Ms i).frame.rel (f i) v /\ v IN (Ms i).frame.world /\ satis (Ms i) v phi}` by metis_tac[CHOICE_DEF] >>
+	fs[])
+     >- (`!i. i IN J ==> (Ms i).frame.world <> {}` by metis_tac[ultraproduct_world] >>
+        `(Ms i).frame.world <> {}` by metis_tac[] >> metis_tac[CHOICE_DEF])
+     >- metis_tac[ultrafilter_def,proper_filter_def,filter_def]
+     >- (`{i | i IN J /\ f i IN (Ms i).frame.world /\
+         ?v. (Ms i).frame.rel (f i) v /\ v IN (Ms i).frame.world /\ satis (Ms i) v phi} ⊆
+	{i | i IN J /\ (Ms i).frame.rel (f i)
+        (if
+           (?v. (Ms i).frame.rel (f i) v /\ v IN (Ms i).frame.world /\ satis (Ms i) v phi)
+        then
+            CHOICE {v | (Ms i).frame.rel (f i) v /\ v IN (Ms i).frame.world /\ satis (Ms i) v phi}
+        else CHOICE (Ms i).frame.world)}`
+	  by (rw[SUBSET_DEF] >>
+	     `{v | (Ms x').frame.rel (f x') v /\ v IN (Ms x').frame.world /\ satis (Ms x') v phi} <> {}`
+	       by (`v' IN {v | (Ms x').frame.rel (f x') v /\ v IN (Ms x').frame.world /\ satis (Ms x') v phi}`
+	             by fs[] >>
+		  metis_tac[MEMBER_NOT_EMPTY]) >>
+             `CHOICE {v | (Ms x').frame.rel (f x') v /\ v IN (Ms x').frame.world /\ satis (Ms x') v phi} IN
+	     {v | (Ms x').frame.rel (f x') v /\ v IN (Ms x').frame.world /\ satis (Ms x') v phi}`
+	       by metis_tac[CHOICE_DEF] >> fs[]) >>
+	`{i | i IN J /\ (Ms i).frame.rel (f i)
+        (if
+           (?v. (Ms i).frame.rel (f i) v /\ v IN (Ms i).frame.world /\ satis (Ms i) v phi)
+        then
+            CHOICE {v | (Ms i).frame.rel (f i) v /\ v IN (Ms i).frame.world /\ satis (Ms i) v phi}
+        else CHOICE (Ms i).frame.world)} ⊆ J` by fs[SUBSET_DEF] >>
+	metis_tac[ultrafilter_def,proper_filter_def,filter_def]) 
+     >- metis_tac[ultraproduct_world]
+     >- (`{v | (Ms i).frame.rel (f i) v /\ v IN (Ms i).frame.world /\ satis (Ms i) v phi} <> {}`
+          by (`v' IN {v | (Ms i).frame.rel (f i) v /\ v IN (Ms i).frame.world /\ satis (Ms i) v phi}` by fs[] >>
+	     metis_tac[MEMBER_NOT_EMPTY]) >>
+	`CHOICE {v | (Ms i).frame.rel (f i) v /\ v IN (Ms i).frame.world /\ satis (Ms i) v phi} IN
+	{v | (Ms i).frame.rel (f i) v /\ v IN (Ms i).frame.world /\ satis (Ms i) v phi}` by metis_tac[CHOICE_DEF] >>
+	fs[])
+     >- (`!i. i IN J ==> (Ms i).frame.world <> {}` by metis_tac[ultraproduct_world] >>
+        `(Ms i).frame.world <> {}` by metis_tac[] >> metis_tac[CHOICE_DEF])
+     >- (`{i | i IN J /\
+        satis (Ms i)
+        (if
+           (?v. (Ms i).frame.rel (f i) v /\ v IN (Ms i).frame.world /\ satis (Ms i) v phi)
+        then
+            CHOICE {v | (Ms i).frame.rel (f i) v /\ v IN (Ms i).frame.world /\ satis (Ms i) v phi}
+        else CHOICE (Ms i).frame.world) phi} IN U`
+	  by (`{i | i IN J /\ f i IN (Ms i).frame.world /\
+             ?v. (Ms i).frame.rel (f i) v /\ v IN (Ms i).frame.world /\ satis (Ms i) v phi} ⊆
+	     {i | i IN J /\ satis (Ms i)
+             (if
+             (?v. (Ms i).frame.rel (f i) v /\ v IN (Ms i).frame.world /\ satis (Ms i) v phi)
+             then
+             CHOICE {v | (Ms i).frame.rel (f i) v /\ v IN (Ms i).frame.world /\ satis (Ms i) v phi}
+             else CHOICE (Ms i).frame.world) phi}`
+	       by (rw[SUBSET_DEF] >>
+	          `{v | (Ms x').frame.rel (f x') v /\ v IN (Ms x').frame.world /\ satis (Ms x') v phi} <> {}`
+		    by (`v' IN {v | (Ms x').frame.rel (f x') v /\ v IN (Ms x').frame.world /\ satis (Ms x') v phi}`
+		          by fs[] >> metis_tac[MEMBER_NOT_EMPTY]) >>
+		  `CHOICE {v | (Ms x').frame.rel (f x') v /\ v IN (Ms x').frame.world /\ satis (Ms x') v phi} IN
+		  {v | (Ms x').frame.rel (f x') v /\ v IN (Ms x').frame.world /\ satis (Ms x') v phi}`
+		    by metis_tac[CHOICE_DEF] >> fs[]) >>
+             `{i | i IN J /\ satis (Ms i)
+             (if
+             (?v. (Ms i).frame.rel (f i) v /\ v IN (Ms i).frame.world /\ satis (Ms i) v phi)
+             then
+             CHOICE {v | (Ms i).frame.rel (f i) v /\ v IN (Ms i).frame.world /\ satis (Ms i) v phi}
+             else CHOICE (Ms i).frame.world) phi} ⊆ J` by fs[SUBSET_DEF] >>
+	     metis_tac[ultrafilter_def,proper_filter_def,filter_def]) >>
+        `{y | (!i. i IN J ==> y i IN (Ms i).frame.world) /\
+              {i | i IN J /\
+                  (if
+                  ?v. (Ms i).frame.rel (f i) v /\ v IN (Ms i).frame.world /\ satis (Ms i) v phi
+                  then
+                  CHOICE {v | (Ms i).frame.rel (f i) v /\ v IN (Ms i).frame.world /\ satis (Ms i) v phi}
+                  else CHOICE (Ms i).frame.world) = y i} IN U} IN (ultraproduct_model U J Ms).frame.world`
+	  by
+	  (`!i. i IN J ==> (Ms i).frame.world <> {}` by metis_tac[ultraproduct_world] >>
+	  `?x.
+            (!i. i IN J ==> x i IN (Ms i).frame.world) /\
+          {y | (!i. i IN J ==> y i IN (Ms i).frame.world) /\
+              {i | i IN J /\
+                  (if
+                  ?v. (Ms i).frame.rel (f i) v /\ v IN (Ms i).frame.world /\ satis (Ms i) v phi
+                  then
+                  CHOICE {v | (Ms i).frame.rel (f i) v /\ v IN (Ms i).frame.world /\ satis (Ms i) v phi}
+                  else CHOICE (Ms i).frame.world) = y i} IN U} =
+          {y | (!i. i IN J ==> y i IN (Ms i).frame.world) /\ {i | i IN J /\ x i = y i} IN U}`
+	  suffices_by metis_tac[ultraproduct_world] >>
+	  qexists_tac
+	  `\i. (if
+             (?v. (Ms i).frame.rel (f i) v /\ v IN (Ms i).frame.world /\ satis (Ms i) v phi)
+             then
+             CHOICE {v | (Ms i).frame.rel (f i) v /\ v IN (Ms i).frame.world /\ satis (Ms i) v phi}
+             else CHOICE (Ms i).frame.world)` >> rw[] (* 2 *)
+	  >- (`{v | (Ms i).frame.rel (f i) v /\ v IN (Ms i).frame.world /\ satis (Ms i) v phi} <> {}`
+	       by (`v' IN {v | (Ms i).frame.rel (f i) v /\ v IN (Ms i).frame.world /\ satis (Ms i) v phi}`
+	             by fs[] >> metis_tac[MEMBER_NOT_EMPTY]) >>
+	     `CHOICE {v | (Ms i).frame.rel (f i) v /\ v IN (Ms i).frame.world /\ satis (Ms i) v phi} IN
+	     {v | (Ms i).frame.rel (f i) v /\ v IN (Ms i).frame.world /\ satis (Ms i) v phi}`
+	       by metis_tac[CHOICE_DEF] >> fs[])
+	  >- metis_tac[CHOICE_DEF]) >>
+	`(\i. (if
+             (?v. (Ms i).frame.rel (f i) v /\ v IN (Ms i).frame.world /\ satis (Ms i) v phi)
+             then
+             CHOICE {v | (Ms i).frame.rel (f i) v /\ v IN (Ms i).frame.world /\ satis (Ms i) v phi}
+             else CHOICE (Ms i).frame.world)) IN
+	{y | (!i. i IN J ==> y i IN (Ms i).frame.world) /\
+              {i | i IN J /\
+                  (if
+                  ?v. (Ms i).frame.rel (f i) v /\ v IN (Ms i).frame.world /\ satis (Ms i) v phi
+                  then
+                  CHOICE {v | (Ms i).frame.rel (f i) v /\ v IN (Ms i).frame.world /\ satis (Ms i) v phi}
+                  else CHOICE (Ms i).frame.world) = y i} IN U}`     
+	  by (rw[] (* 2 *)
+	     >- (Cases_on `?v. (Ms i).frame.rel (f i) v /\ v IN (Ms i).frame.world /\ satis (Ms i) v phi` (* 2 *)
+	        >- (rw[] >>
+		   `{v | (Ms i).frame.rel (f i) v /\ v IN (Ms i).frame.world /\ satis (Ms i) v phi} <> {}`
+	             by (`v' IN {v | (Ms i).frame.rel (f i) v /\ v IN (Ms i).frame.world /\ satis (Ms i) v phi}`
+	                   by fs[] >> metis_tac[MEMBER_NOT_EMPTY]) >>
+		   `CHOICE {v | (Ms i).frame.rel (f i) v /\ v IN (Ms i).frame.world /\ satis (Ms i) v phi} IN
+	           {v | (Ms i).frame.rel (f i) v /\ v IN (Ms i).frame.world /\ satis (Ms i) v phi}`
+	             by metis_tac[CHOICE_DEF] >> fs[])
+		>- (rw[] >> metis_tac[CHOICE_DEF,ultraproduct_world]))
+	     >- metis_tac[ultrafilter_def,proper_filter_def,filter_def]) >> metis_tac[])
+
+
+
+
+
+
+  
+
+
+val ultraproduct_world_NOT_EMPTY = store_thm(
+  "ultraproduct_world_NOT_EMPTY",
+  ``!U J MS v. ultrafilter U J ==> v IN (ultraproduct_model U J MS).frame.world ==> v <> {}``,
+  rw[ultraproduct_def,ultraproduct_model_def, models2worlds_def] >> metis_tac[prop_A_16,EMPTY_NOT_IN_partition]);
+
+val ultraproduct_world = store_thm(
+  "ultraproduct_world",
+  ``!U J MS.
+    ultrafilter U J ==>
+       (!v.
+           v ∈ (ultraproduct_model U J MS).frame.world <=>
+               (!i. i IN J ==> (MS i).frame.world <> {}) /\
+               (∃x.
+                   (∀i. i ∈ J ⇒ x i ∈ (MS i).frame.world) /\
+                   v = {y | (∀i. i ∈ J ⇒ y i ∈ (MS i).frame.world) /\ {i | i ∈ J ∧ x i = y i} ∈ U}))``,
+  rw[ultraproduct_def,ultraproduct_model_def, models2worlds_def,partition_def,Uequiv_def,Cart_prod_def] >> rw[EQ_IMP_THM] (* 3 *)
+  >- metis_tac[MEMBER_NOT_EMPTY]
+  >> qexists_tac `x` >> rw[EXTENSION,EQ_IMP_THM] >> metis_tac[]);
+
+  
+val ultraproduct_rel = save_thm(
+  "ultraproduct_rel",
+  ``(ultraproduct_model U J MS).frame.rel w v``
+    |> SIMP_CONV (srw_ss()) [ultraproduct_def,ultraproduct_model_def, models2worlds_def,partition_def,Uequiv_def,Cart_prod_def])
+
+val ultraproduct_valt = save_thm(
+  "ultraproduct_valt",
+  ``v IN (ultraproduct_model U J MS).valt p``
+    |> SIMP_CONV (srw_ss()) [ultraproduct_def,ultraproduct_model_def, models2worlds_def,partition_def,Uequiv_def,Cart_prod_def])
+
+
+
 (*
-val ultraproduct_worlds = store_thm(
-  "ultraproduct_worlds",
-  ``v ∈ (ultraproduct_model U J Ms).frame.world <=>
-    ?f. ...
-
-val _ = hide "I"
-
-val _ = reveal "I"
-val prop_2_71 = store_thm(
-  "prop_2_71",
-  ``!U I MS. (!i. i IN I ==> (MS i) = M) /\ ultrafilter U I ==>
-         !phi w. w IN M.frame.world ==>
-         (satis (ultraproduct_model U I MS) {fw | Uequiv U I (models2worlds MS) (\i.w) fw} phi <=>  satis M w phi)``,
-  strip_tac >> strip_tac >> strip_tac >> strip_tac >> Induct_on `phi` >> rw[] (* 5 *)
-  >- (rw[EQ_IMP_THM,satis_def] (* 4 *)
-     >- (rw[ultraproduct_model_def,ultraproduct_def] >> rw[partition_def] >>
-        qexists_tac `\i.w` >> rw[] (* 2 *)
-	>- (rw[Cart_prod_def] >> rw[models2worlds_def])
-	>- (rw[Uequiv_def] >> simp[EXTENSION] >> metis_tac[]))
-     >- (rw[ultraproduct_model_def] >> qexists_tac `\i.w` >> rw[] (* 2 *)
-        >- (`(Uequiv U I' (models2worlds MS)) equiv_on (Cart_prod I' (models2worlds MS))` by metis_tac[prop_A_16] >>
-	   fs[equiv_on_def] >>
-	   `(λi. w) IN (Cart_prod I' (models2worlds MS))` suffices_by metis_tac[] >>
-	   rw[models2worlds_def,Cart_prod_def])
-	>- (`!i. i IN I' ==> w IN ((MS i).valt) a` by rw[] >>
-	   `{i | i ∈ I' ∧ w ∈ (MS i).valt a} = I'` by (simp[EXTENSION] >> metis_tac[]) >>
-	   fs[ultrafilter_def,proper_filter_def,filter_def]))
-     >- (fs[ultraproduct_model_def,models2worlds_def,ultraproduct_def] >> fs[Uequiv_def] >> fs[Cart_prod_def] >>
-        `I' <> {}` by fs[ultrafilter_def,proper_filter_def,filter_def] >>
-	`?i. i IN I'` by metis_tac[MEMBER_NOT_EMPTY] >>
-	metis_tac[])
-     >- (fs[ultraproduct_model_def,models2worlds_def,ultraproduct_def] >> fs[Uequiv_def,Cart_prod_def] >>
-        `({i | i ∈ I' ∧ w = f i} INTER {i | i ∈ I' ∧ f i ∈ (MS i).valt a}) IN U` by metis_tac[ultrafilter_def,proper_filter_def,filter_def] >>
-	`{i | i ∈ I' ∧ w = f i} INTER {i | i ∈ I' ∧ f i ∈ (MS i).valt a} <> {}` by metis_tac[EMPTY_NOTIN_ultrafilter] >>
-	`?i. i IN ({i | i ∈ I' ∧ w = f i} INTER {i | i ∈ I' ∧ f i ∈ (MS i).valt a})` by metis_tac[MEMBER_NOT_EMPTY] >>
-	fs[] >> metis_tac[]))
-  >- rw[satis_def,EQ_IMP_THM]
-  >- rw[satis_def,EQ_IMP_THM]
-  >- (rw[satis_def,EQ_IMP_THM] (* 2 *)
-     >- (rw[ultraproduct_model_def,ultraproduct_def] >> rw[partition_def,Uequiv_def,Cart_prod_def,models2worlds_def] >>
-        qexists_tac `\i.w` >> rw[] >> simp[EXTENSION] >> metis_tac[])
-     >- (fs[ultraproduct_model_def,ultraproduct_def,partition_def,Uequiv_def,Cart_prod_def,models2worlds_def] >>
-        `{y |
-        (∀i. i ∈ I' ⇒ y i ∈ (MS i).frame.world) ∧ ultrafilter U I' ∧
-        (∀i. i ∈ I' ⇒ (MS i).frame.world ≠ ∅) ∧
-        (∀i. i ∈ I' ⇒ x i ∈ (MS i).frame.world) ∧
-        (∀i. i ∈ I' ⇒ y i ∈ (MS i).frame.world) ∧
-        {i | i ∈ I' ∧ x i = y i} ∈ U} <> {}`
-            by (`x IN {y |
-                         (∀i. i ∈ I' ⇒ y i ∈ (MS i).frame.world) ∧ ultrafilter U I' ∧
-                         (∀i. i ∈ I' ⇒ (MS i).frame.world ≠ ∅) ∧
-                         (∀i. i ∈ I' ⇒ x i ∈ (MS i).frame.world) ∧
-                         (∀i. i ∈ I' ⇒ y i ∈ (MS i).frame.world) ∧
-                         {i | i ∈ I' ∧ x i = y i} ∈ U}` suffices_by metis_tac[MEMBER_NOT_EMPTY] >>
-		fs[] >> rw[] (* 2 *)
-		>- metis_tac[MEMBER_NOT_EMPTY]
-		>- metis_tac[ultrafilter_def,proper_filter_def,filter_def]) >>
-	`{fw |
-        ultrafilter U I' ∧ (∀i. i ∈ I' ⇒ (MS i).frame.world ≠ ∅) ∧
-        (∀i. i ∈ I' ⇒ w ∈ (MS i).frame.world) ∧
-        (∀i. i ∈ I' ⇒ fw i ∈ (MS i).frame.world) ∧
-        {i | i ∈ I' ∧ w = fw i} ∈ U} <> {}` by metis_tac[] >>
-	`?fw. fw IN {fw |
-                    ultrafilter U I' ∧ (∀i. i ∈ I' ⇒ (MS i).frame.world ≠ ∅) ∧
-                    (∀i. i ∈ I' ⇒ w ∈ (MS i).frame.world) ∧
-                    (∀i. i ∈ I' ⇒ fw i ∈ (MS i).frame.world) ∧
-                    {i | i ∈ I' ∧ w = fw i} ∈ U}` by metis_tac[MEMBER_NOT_EMPTY] >> fs[] >>
-	`{i | i ∈ I' ∧ w = fw i} <> {}` by metis_tac[EMPTY_NOTIN_ultrafilter] >>
-	`?i. i IN {i | i ∈ I' ∧ w = fw i}` by metis_tac[MEMBER_NOT_EMPTY] >>
-	fs[] >> metis_tac[]))
-  >- rw[satis_def,EQ_IMP_THM] (* 4 *)
-     >- (rw[ultraproduct_model_def,ultraproduct_def] >> rw[partition_def,Uequiv_def,Cart_prod_def,models2worlds_def] >>
-        qexists_tac `\i.w` >> rw[] >> simp[EXTENSION] >> metis_tac[])
-     >-
-
-
-
-
-
-rw[satis_def] >> pop_assum (ASSUME_TAC o GSYM) >> simp[]
 
 
 
@@ -132,165 +485,106 @@ rw[satis_def] >> pop_assum (ASSUME_TAC o GSYM) >> simp[]
 
 
 
-
-rw[ultraproduct_model_def] >> simp[PULL_EXISTS] >> rw[ultraproduct_def,partition_def,Cart_prod_def] >>
-        simp[PULL_EXISTS] >>
-	map_every qexists_tac [`\i.w`,`\i.v`,`\i.v`] >> rw[] (* 6 *)
-	>- (`(Uequiv U I' (models2worlds MS)) equiv_on (Cart_prod I' (models2worlds MS))` by metis_tac[prop_A_16] >>
-	   fs[equiv_on_def] >>
-	   `(λi. w) IN (Cart_prod I' (models2worlds MS))` suffices_by metis_tac[] >>
-	   rw[models2worlds_def,Cart_prod_def])
-	>- rw[models2worlds_def]
-	>- (`(Uequiv U I' (models2worlds MS)) equiv_on (Cart_prod I' (models2worlds MS))` by metis_tac[prop_A_16] >>
-	   fs[equiv_on_def] >>
-	   `(λi. v) IN (Cart_prod I' (models2worlds MS))` suffices_by metis_tac[] >>
-	   rw[models2worlds_def,Cart_prod_def])
-	>- (`{i | i ∈ I' ∧ (MS i).frame.rel w v} = I'` suffices_by metis_tac[ultrafilter_def,proper_filter_def,filter_def] >> simp[EXTENSION] >> `I' <> {}` by metis_tac[ultrafilter_def,proper_filter_def,filter_def] >>
-	   metis_tac[MEMBER_NOT_EMPTY])
-	>- rw[models2worlds_def
-
+val ultraproduct_world_constant = store_thm(
+  "ultraproduct_world_constant",
+  ``!U J MS w.
+  ultrafilter U J ⇒
+  (∀i. i ∈ J ⇒ MS i = M) ⇒
+  ({fw | Uequiv U J (models2worlds MS) (λi. w) fw} ∈ (ultraproduct_model U J MS).frame.world
+  <=> w ∈ M.frame.world)``,
+  rw[EQ_IMP_THM] 
+  >- (`?i. i IN J`
+       by metis_tac[ultrafilter_def,proper_filter_def,filter_def,MEMBER_NOT_EMPTY] >>
+     `{fw | Uequiv U J (models2worlds MS) (λi. w) fw} <> {}`
+       by metis_tac[ultraproduct_world_NOT_EMPTY] >> fs[ultraproduct_world] >>
+     fs[Uequiv_def,models2worlds_def,Cart_prod_def] >>
+     `?a. a IN {fw |
+       ultrafilter U J ∧ (∀i. i ∈ J ⇒ (MS i).frame.world ≠ ∅) ∧
+       (∀i. i ∈ J ⇒ w ∈ (MS i).frame.world) ∧
+       (∀i. i ∈ J ⇒ fw i ∈ (MS i).frame.world) ∧
+       {i | i ∈ J ∧ w = fw i} ∈ U}` by metis_tac[MEMBER_NOT_EMPTY] >> fs[] >> metis_tac[])
+  >- (rw[ultraproduct_world] (* 2 *)
+     >- metis_tac[MEMBER_NOT_EMPTY]
+     >- (qexists_tac `\i.w` >> rw[Uequiv_def,models2worlds_def,Cart_prod_def] >>
+        simp[EXTENSION] >> metis_tac[])));
 
 
 
 val prop_2_71 = store_thm(
   "prop_2_71",
-  ``!U I MS. (!i. i IN I ==> (MS i) = M) /\ ultrafilter U I ==>
-         !phi w. satis M w phi <=> satis (ultraproduct_model U I MS) {fw | Uequiv U I (models2worlds MS) (\i.w) fw} phi``,
+  ``!U J MS. (!i. i IN J ==> (MS i) = M) /\ ultrafilter U J ==>
+         !phi w. satis (ultraproduct_model U J MS) {fw | Uequiv U J (models2worlds MS) (\i.w) fw} phi <=> satis M w phi``,
   strip_tac >> strip_tac >> strip_tac >> strip_tac >> Induct_on `phi` >> rw[] (* 5 *)
-  >- (rw[EQ_IMP_THM,satis_def] (* 4 *)
-     >- (rw[ultraproduct_model_def,ultraproduct_def] >> rw[partition_def] >>
-        qexists_tac `\i.w` >> rw[] (* 2 *)
-	>- (rw[Cart_prod_def] >> rw[models2worlds_def])
-	>- (rw[Uequiv_def] >> simp[EXTENSION] >> metis_tac[]))
-     >- (rw[ultraproduct_model_def] >> qexists_tac `\i.w` >> rw[] (* 2 *)
-        >- (`(Uequiv U I' (models2worlds MS)) equiv_on (Cart_prod I' (models2worlds MS))` by metis_tac[prop_A_16] >>
-	   fs[equiv_on_def] >>
-	   `(λi. w) IN (Cart_prod I' (models2worlds MS))` suffices_by metis_tac[] >>
-	   rw[models2worlds_def,Cart_prod_def])
-	>- (`!i. i IN I' ==> w IN ((MS i).valt) a` by rw[] >>
-	   `{i | i ∈ I' ∧ w ∈ (MS i).valt a} = I'` by (simp[EXTENSION] >> metis_tac[]) >>
-	   fs[ultrafilter_def,proper_filter_def,filter_def]))
-     >- (fs[ultraproduct_model_def,models2worlds_def,ultraproduct_def] >> fs[Uequiv_def] >> fs[Cart_prod_def] >>
-        `I' <> {}` by fs[ultrafilter_def,proper_filter_def,filter_def] >>
-	`?i. i IN I'` by metis_tac[MEMBER_NOT_EMPTY] >>
-	metis_tac[])
-     >- (fs[ultraproduct_model_def,models2worlds_def,ultraproduct_def] >> fs[Uequiv_def,Cart_prod_def] >>
-        `({i | i ∈ I' ∧ w = f i} INTER {i | i ∈ I' ∧ f i ∈ (MS i).valt a}) IN U` by metis_tac[ultrafilter_def,proper_filter_def,filter_def] >>
-	`{i | i ∈ I' ∧ w = f i} INTER {i | i ∈ I' ∧ f i ∈ (MS i).valt a} <> {}` by metis_tac[EMPTY_NOTIN_ultrafilter] >>
-	`?i. i IN ({i | i ∈ I' ∧ w = f i} INTER {i | i ∈ I' ∧ f i ∈ (MS i).valt a})` by metis_tac[MEMBER_NOT_EMPTY] >>
-	fs[] >> metis_tac[]))
+  >- (rw[satis_def,EQ_IMP_THM] (* 4 *)
+     >- metis_tac[ultraproduct_world_constant]
+     >- (fs[ultraproduct_valt,Uequiv_def] >>
+        `({i | i ∈ J ∧ w = f i} INTER {i | i ∈ J ∧ f i ∈ (MS i).valt a}) IN U`
+	  by metis_tac[ultrafilter_def,proper_filter_def,filter_def] >>
+	`{i | i ∈ J ∧ w = f i} ∩ {i | i ∈ J ∧ f i ∈ (MS i).valt a} <> {}` by metis_tac[EMPTY_NOTIN_ultrafilter] >>
+	`?i. i IN {i | i ∈ J ∧ w = f i} ∩ {i | i ∈ J ∧ f i ∈ (MS i).valt a}` by metis_tac[MEMBER_NOT_EMPTY] >> fs[] >> metis_tac[])
+     >- (simp[ultraproduct_world] >> rw[] (* 2 *)
+        >- metis_tac[MEMBER_NOT_EMPTY]
+	>- (qexists_tac `\i.w` >> rw[] >>
+	   rw[Uequiv_def,models2worlds_def,Cart_prod_def] >> simp[EXTENSION] >> metis_tac[]))
+     >- (simp[ultraproduct_valt] >> qexists_tac `\i.w` >> rw[] (* 2 *)
+        >- (rw[Uequiv_def,Cart_prod_def,models2worlds_def] 
+	   >- metis_tac[MEMBER_NOT_EMPTY]
+	   >- metis_tac[ultrafilter_def,proper_filter_def,filter_def])
+	>- (`{i | i ∈ J ∧ w ∈ (MS i).valt a} = J` suffices_by
+	   metis_tac[ultrafilter_def,proper_filter_def,filter_def] >> simp[EXTENSION] >>
+	   metis_tac[])))
   >- rw[satis_def,EQ_IMP_THM]
   >- rw[satis_def,EQ_IMP_THM]
-  >- (rw[satis_def,EQ_IMP_THM] (* 2 *)
-     >- (rw[ultraproduct_model_def,ultraproduct_def] >> rw[partition_def,Uequiv_def,Cart_prod_def,models2worlds_def] >>
-        qexists_tac `\i.w` >> rw[] >> simp[EXTENSION] >> metis_tac[])
-     >- (fs[ultraproduct_model_def,ultraproduct_def,partition_def,Uequiv_def,Cart_prod_def,models2worlds_def] >>
-        `{y |
-        (∀i. i ∈ I' ⇒ y i ∈ (MS i).frame.world) ∧ ultrafilter U I' ∧
-        (∀i. i ∈ I' ⇒ (MS i).frame.world ≠ ∅) ∧
-        (∀i. i ∈ I' ⇒ x i ∈ (MS i).frame.world) ∧
-        (∀i. i ∈ I' ⇒ y i ∈ (MS i).frame.world) ∧
-        {i | i ∈ I' ∧ x i = y i} ∈ U} <> {}`
-            by (`x IN {y |
-                         (∀i. i ∈ I' ⇒ y i ∈ (MS i).frame.world) ∧ ultrafilter U I' ∧
-                         (∀i. i ∈ I' ⇒ (MS i).frame.world ≠ ∅) ∧
-                         (∀i. i ∈ I' ⇒ x i ∈ (MS i).frame.world) ∧
-                         (∀i. i ∈ I' ⇒ y i ∈ (MS i).frame.world) ∧
-                         {i | i ∈ I' ∧ x i = y i} ∈ U}` suffices_by metis_tac[MEMBER_NOT_EMPTY] >>
-		fs[] >> rw[] (* 2 *)
-		>- metis_tac[MEMBER_NOT_EMPTY]
-		>- metis_tac[ultrafilter_def,proper_filter_def,filter_def]) >>
-	`{fw |
-        ultrafilter U I' ∧ (∀i. i ∈ I' ⇒ (MS i).frame.world ≠ ∅) ∧
-        (∀i. i ∈ I' ⇒ w ∈ (MS i).frame.world) ∧
-        (∀i. i ∈ I' ⇒ fw i ∈ (MS i).frame.world) ∧
-        {i | i ∈ I' ∧ w = fw i} ∈ U} <> {}` by metis_tac[] >>
-	`?fw. fw IN {fw |
-                    ultrafilter U I' ∧ (∀i. i ∈ I' ⇒ (MS i).frame.world ≠ ∅) ∧
-                    (∀i. i ∈ I' ⇒ w ∈ (MS i).frame.world) ∧
-                    (∀i. i ∈ I' ⇒ fw i ∈ (MS i).frame.world) ∧
-                    {i | i ∈ I' ∧ w = fw i} ∈ U}` by metis_tac[MEMBER_NOT_EMPTY] >> fs[] >>
-	`{i | i ∈ I' ∧ w = fw i} <> {}` by metis_tac[EMPTY_NOTIN_ultrafilter] >>
-	`?i. i IN {i | i ∈ I' ∧ w = fw i}` by metis_tac[MEMBER_NOT_EMPTY] >>
-	fs[] >> metis_tac[]))
-  >- rw[satis_def,EQ_IMP_THM] (* 4 *)
-     >- (rw[ultraproduct_model_def,ultraproduct_def] >> rw[partition_def,Uequiv_def,Cart_prod_def,models2worlds_def] >>
-        qexists_tac `\i.w` >> rw[] >> simp[EXTENSION] >> metis_tac[])
-     >- (fs[ultraproduct_model_def] >> simp[PULL_EXISTS] >> fs[ultraproduct_def,partition_def,Cart_prod_def] >>
-        simp[PULL_EXISTS] >>
-	map_every qexists_tac [`\i.w`,`\i.v`,`\i.v`] >> rw[] (* 6 *)
-	>- (`(Uequiv U I' (models2worlds MS)) equiv_on (Cart_prod I' (models2worlds MS))` by metis_tac[prop_A_16] >>
-	   fs[equiv_on_def] >>
-	   `(λi. w) IN (Cart_prod I' (models2worlds MS))` suffices_by metis_tac[] >>
-	   rw[models2worlds_def,Cart_prod_def])
-	>- rw[models2worlds_def]
-	>- (`(Uequiv U I' (models2worlds MS)) equiv_on (Cart_prod I' (models2worlds MS))` by metis_tac[prop_A_16] >>
-	   fs[equiv_on_def] >>
-	   `(λi. v) IN (Cart_prod I' (models2worlds MS))` suffices_by metis_tac[] >>
-	   rw[models2worlds_def,Cart_prod_def])
-	>- (`{i | i ∈ I' ∧ (MS i).frame.rel w v} = I'` suffices_by metis_tac[ultrafilter_def,proper_filter_def,filter_def] >> simp[EXTENSION] >> `I' <> {}` by metis_tac[ultrafilter_def,proper_filter_def,filter_def] >>
-	   metis_tac[MEMBER_NOT_EMPTY])
-	>- rw[models2worlds_def]
-	>- (`{y | (∀i. i ∈ I' ⇒ y i ∈ models2worlds MS i) ∧ Uequiv U I' (models2worlds MS) (λi. v) y} =
-	   {fw | Uequiv U I' (models2worlds MS) (λi. v) fw}` suffices_by metis_tac[] >>
-	   simp[EXTENSION] >>
-	   `!x. Uequiv U I' (models2worlds MS) (λi. v) x ==> (∀i. i ∈ I' ⇒ x i ∈ models2worlds MS i)`
-	   suffices_by metis_tac[] >>
-	   rw[Uequiv_def,models2worlds_def,Cart_prod_def]))
-     >- (fs[ultraproduct_model_def,models2worlds_def,ultraproduct_def] >> fs[Uequiv_def,Cart_prod_def] >>
-        `I' <> {}` by metis_tac[ultrafilter_def,proper_filter_def,filter_def] >>
-	`?i. i IN I'` by metis_tac[MEMBER_NOT_EMPTY] >>
+  >- (rw[satis_def,EQ_IMP_THM] (* 2 *) >> metis_tac[ultraproduct_world_constant])
+  >- rw[satis_def,EQ_IMP_THM]
+     >- metis_tac[ultraproduct_world_constant]
+     >- `(!i. i IN J ==> (MS i).frame.world <> {}) /\
+         ?x.
+            (!i. i IN J ==> x i IN (MS i).frame.world) /\
+            v =
+            {y |
+             (!i. i IN J ==> y i IN (MS i).frame.world) /\
+             {i | i IN J /\ x i = y i} IN U}` by metis_tac[ultraproduct_world] >> fs[] >>
+	Q.UNDISCH_THEN `{y |
+       (!i. i IN J ==> y i IN (MS i).frame.world) /\
+       {i | i IN J /\ x i = y i} IN U} IN
+      (ultraproduct_model U J MS).frame.world` (K ALL_TAC) >>
+      fs[ultraproduct_rel] >>
+      Q.UNDISCH_THEN `v =
+       {y |
+        (!i. i IN J ==> y i IN (MS i).frame.world) /\
+        {i | i IN J /\ x i = y i} IN U}` (K ALL_TAC) >>
+      fs[Uequiv_def]
+
+
+
+
+
+
+`?w'. v = {fw | Uequiv U J (models2worlds MS) (\i. w') fw}`
+           by (simp[EXTENSION, Uequiv_def]  >>
+               drule_then (fn th => fs[th]) ultraproduct_world >> rfs[] >>
+	       rw[] >> simp[Cart_prod_def, models2worlds_def] >>
+	       `!i. i IN J ==> ?x. x IN M.frame.world`
+	         by metis_tac[MEMBER_NOT_EMPTY] >>
+	       pop_assum (SUBST1_TAC o EQT_INTRO) >> simp[]
+
+
+        `w' IN M.frame.world`
+	   by ((* use ultraproduct_world_constant *) cheat) 
+	`M.frame.rel w w'`
+	   by (fs[ultraproduct_rel] >>
+	       REV_FULL_SIMP_TAC (srw_ss() ++ boolSimps.CONJ_ss)[] >> cheat)
 	metis_tac[])
-     >- 
 
 
 
-
-
-
-
-
-
-
-
-
-`v IN (ultraproduct_model U I' MS).frame.world ==>
-        ∃v.
-         M.frame.rel w v ∧ v ∈ M.frame.world ∧
-         satis (ultraproduct_model U I' MS)
-         {fw | Uequiv U I' (models2worlds MS) (λi. v) fw} phi` suffices_by metis_tac[] >>
-	
-
-
-
-fs[ultraproduct_model_def] >>
-        `{i | i ∈ I' ∧ (MS i).frame.rel (f i) (g i)} <> {}` by metis_tac[EMPTY_NOTIN_ultrafilter] >>
-	fs[Uequiv_def,ultraproduct_def,Cart_prod_def] >>
-	`({i | i ∈ I' ∧ w = f i} INTER {i | i ∈ I' ∧ (MS i).frame.rel (f i) (g i)}) IN U`
-	    by metis_tac[ultrafilter_def,proper_filter_def,filter_def] >>
-	`?i. i IN ({i | i ∈ I' ∧ w = f i} INTER {i | i ∈ I' ∧ (MS i).frame.rel (f i) (g i)})`
-	    by metis_tac[MEMBER_NOT_EMPTY,EMPTY_NOTIN_ultrafilter] >>
-	fs[] >> qexists_tac `g i'` >> rw[] (* 3 *)
-	>- metis_tac[]
-	>- (fs[partition_def,Uequiv_def] >> fs[Cart_prod_def] >> metis_tac[models2worlds_def])
-	>- `v = {fw |
-                (∀i''. i'' ∈ I' ⇒ g i' ∈ models2worlds MS i'') ∧
-                (∀i. i ∈ I' ⇒ fw i ∈ models2worlds MS i) ∧
-                {i | i ∈ I' ∧ g i' = fw i} ∈ U}` suffices_by metis_tac[] >>
-           fs[partition_def,Uequiv_def,Cart_prod_def] >>
-	   `g IN {y |
-                 (∀i. i ∈ I' ⇒ y i ∈ models2worlds MS i) ∧ ultrafilter U I' ∧
-                 (∀i. i ∈ I' ⇒ models2worlds MS i ≠ ∅) ∧
-                 (∀i. i ∈ I' ⇒ x' i ∈ models2worlds MS i) ∧
-                 (∀i. i ∈ I' ⇒ y i ∈ models2worlds MS i) ∧
-                 {i | i ∈ I' ∧ x' i = y i} ∈ U}` by metis_tac[] >> fs[] >>
-	   rw[EXTENSION,EQ_IMP_THM] (* 3 *)
-	   >- metis_tac[models2worlds_def]
-	   >- 
 	   
 *)	
 
-  
+
+
+*)
 
 
 val _ = export_theory();
